proof

src/computation.lean
@@ -5,17 +5,71 @@ import
   computability.partrec_code
   computability.halting
   data.pfun
-  deduction semantics cltheory arithmetic
+  deduction semantics lindenbaum arithmetic
 
 open encodable denumerable roption
 
+namespace nat.primrec
+
+inductive code : Type
+| zero : code
+| succ : code
+| left : code
+| right : code
+| pair : code → code → code
+| comp : code → code → code
+| prec : code → code → code
+
+namespace code
+
+def eval : code → ℕ → ℕ
+| zero         := λ x, 0
+| succ         := nat.succ
+| left         := λ n : ℕ, n.unpair.1
+| right        := λ n : ℕ, n.unpair.2
+| (pair cf cg) := λ n, nat.mkpair (eval cf n) (eval cg n)
+| (comp cf cg) := λ n, eval cf (eval cg n)
+| (prec cf cg) := nat.unpaired (λ a n : ℕ, n.elim (eval cf a) (λ y i, eval cg (a.mkpair (y.mkpair i))))
+
+theorem exists_code {f : ℕ → ℕ} : nat.primrec f ↔ ∃ c : code, eval c = f := ⟨λ h,
+begin
+  induction h,
+  case nat.primrec.zero { refine ⟨zero, rfl⟩ },
+  case nat.primrec.succ { exact ⟨succ, rfl⟩ },
+  case nat.primrec.left { exact ⟨left, rfl⟩ },
+  case nat.primrec.right { exact ⟨right, rfl⟩ },  
+  case nat.primrec.pair : f g pf pg hf hg 
+  { rcases hf with ⟨cf, rfl⟩, rcases hg with ⟨cg, rfl⟩, refine ⟨pair cf cg, rfl⟩ },
+  case nat.primrec.comp : f g pf pg hf hg {
+    rcases hf with ⟨cf, rfl⟩, rcases hg with ⟨cg, rfl⟩,
+    exact ⟨comp cf cg, rfl⟩ },
+  case nat.primrec.prec : f g pf pg hf hg {
+    rcases hf with ⟨cf, rfl⟩, rcases hg with ⟨cg, rfl⟩,
+    exact ⟨prec cf cg, rfl⟩ }
+end, λ h,
+begin
+  rcases h with ⟨c, rfl⟩, induction c,
+  case nat.primrec.code.zero { exact nat.primrec.zero },
+  case nat.primrec.code.succ { exact nat.primrec.succ },
+  case nat.primrec.code.left { exact nat.primrec.left },
+  case nat.primrec.code.right { exact nat.primrec.right },
+  case nat.primrec.code.pair : cf cg pf pg { exact pf.pair pg },
+  case nat.primrec.code.comp : cf cg pf pg { exact pf.comp pg },
+  case nat.primrec.code.prec : cf cg pf pg { exact pf.prec pg },
+end⟩
+
+end code
+
+end nat.primrec
+
 namespace fopl
+
+namespace arithmetic
 
 namespace LC
 
-
 inductive langf : ℕ → Type
-| fn₁ : nat.partrec.code → langf 1
+| fn₁ : nat.primrec.code → langf 1
 | pair : langf 2
 notation `*fn₁` n := langf.fn₁ n
 notation `*fn₂` n := langf.fn₂ n
@@ -26,24 +80,42 @@ end LC
 
 def LC : language := ⟨LC.langf, LC.langp⟩
 
-namespace LC
-open nat.partrec
+open nat.primrec
 
-@[reducible] def symbol.fn₁ (c : nat.partrec.code) : term (LA + LC) → term (LA + LC) := λ x, vecterm.app (sum.inr (*fn₁ c)) x
-prefix `Ḟ₁ `:max := symbol.fn₁
+@[reducible] def symbol.fn₁ (c : nat.primrec.code) : term (LA + LC) → term (LA + LC) := λ x, vecterm.app (sum.inr (*fn₁ c)) x
+prefix `Ḟ `:max := symbol.fn₁
 
-@[reducible] def symbol.pair : term (LA + LC) → term (LA + LC) → term (LA + LC) :=
-λ x y, vecterm.app (sum.inr langf.pair) (x ::: y)
+@[reducible] def pair : term (LA + LC) → term (LA + LC) → term (LA + LC) :=
+λ x y, vecterm.app (sum.inr LC.langf.pair) (x ::: y)
 
-inductive computation : theory (LA + LC)
-| zero : computation (∀̇ ((Ḟ₁ code.zero) #0 =̇ Ż))
-| succ : computation (∀̇ ((Ḟ₁ code.succ) #0 =̇ Ṡ #0))
-| pair : ∀ (c₁ c₂ : code), computation (∀̇ ((Ḟ₁ (code.pair c₁ c₂)) #0 =̇ symbol.pair (Ḟ₁ c₁ $ #0) (Ḟ₁ c₂ $ #0)))
-| prec : 
+inductive Prim : theory (LA + LC)
+| zero   : Prim ∀̇ (Ḟ code.zero #0 =̇ Ż)
+| succ   : Prim ∀̇ (Ḟ code.succ #0 =̇ Ṡ #0)
+| right  : Prim ∀̇ (Ḟ code.right (pair #0 #1) =̇ #0)
+| left   : Prim ∀̇ (Ḟ code.left (pair #0 #1) =̇ #1)
+| pair   : ∀ (c₁ c₂ : code), Prim ∀̇ (Ḟ (code.pair c₁ c₂) #0 =̇ pair (Ḟ c₁ $ #0) (Ḟ c₂ $ #0))
+| comp   : ∀ (c₁ c₂ : code), Prim ∀̇ (Ḟ (code.comp c₁ c₂) #0 =̇ Ḟ c₁ (Ḟ c₂ $ #0))
+| prec_z : ∀ (c₁ c₂ : code), Prim ∀̇ (Ḟ (code.prec c₁ c₂) (pair #0 Ż) =̇ Ḟ c₁ #0)
+| prec_s : ∀ (c₁ c₂ : code),
+    Prim ∀̇ ∀̇ (Ḟ (code.prec c₁ c₂) (pair #0 (Ṡ #1)) =̇ Ḟ c₂ (pair #0 (Ḟ (code.prec c₁ c₂) (pair #0 #1))))
 
+theorem complete (T : theory LA) [extend 𝐐 T] (f : ℕ → ℕ) (h : primrec f) : ∃ c : code, ∀ n m : ℕ,
+  f n = m → Prim ⊢ Ḟ c (numeral n) =̇ (numeral m) :=
+begin
+  suffices :
+    ∀ c : code, ∀ n m : ℕ, c.eval n = m → Prim ⊢ Ḟ c (numeral n) =̇ (numeral m),
+  { rcases code.exists_code.mp (primrec.nat_iff.mp h) with ⟨c, rfl⟩,
+    refine ⟨c, this c⟩ },
+  intros c, induction c,
+  case code.zero { simp[code.eval], rintros n m rfl, refine (provable.AX Prim.zero).fal_subst (numeral n) },
+  case code.succ { simp[code.eval], rintros n m rfl, refine (provable.AX Prim.succ).fal_subst (numeral n) },
+  case code.comp : cf cg hf hg { simp[code.eval], rintros n m rfl,
+    have : Prim ⊢ Ḟ (cf.comp cg) (numeral n) =̇ Ḟ cf (Ḟ cg (numeral n)), from (provable.AX $ Prim.comp cf cg).fal_subst (numeral n),
+    sorry }, sorry,
+  --rcases code.exists_code.mp (primrec.nat_iff.mp h) with ⟨c, rfl⟩,
+  --use c,
+end
 
-notation `𝐐` := robinson
-
-end LC
+end arithmetic
 
 end fopl
