src/proof.lean
@@ -1,0 +1,87 @@
+import deduction semantics lindenbaum
+open encodable
+
+namespace fopl
+variables {L : language.{0}} 
+
+inductive proof : ℕ → formula L → Type
+| p1 : ∀ {n} p q, proof n (p →̇ q →̇ p)
+| p2 : ∀ {n} p q r, proof n ((p →̇ q →̇ r) →̇ (p →̇ q) →̇ p →̇ r)
+| p3 : ∀ {n} p q, proof n ((¬̇p →̇ ¬̇q) →̇ q →̇ p)
+| q1 : ∀ {n} p t, proof n (∀̇ p →̇ p.rew ι[0 ⇝ t])
+| q2 : ∀ {n} p q, proof n (∀̇ (p →̇ q) →̇ ∀̇ p →̇∀̇ q)
+| q3 : ∀ {n} p, proof n (p →̇ ∀̇ (p^1))
+| e1 : ∀ {n} t, proof n (t =̇ t)
+| e2 : ∀ {n} t₁ t₂, proof n (t₁ =̇ t₂ →̇ t₂ =̇ t₁)
+| e3 : ∀ {n} t₁ t₂ t₃, proof n (t₁ =̇ t₂ →̇ t₂ =̇ t₃ →̇ t₁ =̇ t₃)
+| e4 : ∀ {n m} f (v₁ v₂ : vecterm L m), proof n (v₁ ≡̇ v₂ →̇ vecterm.app f v₁ =̇ vecterm.app f v₂)
+| e5 : ∀ {n m} r (v₁ v₂ : vecterm L m), proof n (v₁ ≡̇ v₂ →̇ formula.app r v₁ →̇ formula.app r v₂)
+| GE : ∀ {n p}, proof (n + 1) p → proof n (∀̇ p)
+| MP : ∀ {n p q}, proof n (p →̇ q) → proof n p → proof n q
+| AX : ∀ {n} p, proof n p
+
+variables [primcodable (formula L)] 
+
+@[simp] def proof.wellformed (T : theory L) [prm : ∀ i : ℕ, primrec_theory (T^i)] :
+  ∀ {n} {p : formula L}, proof n p → bool
+| _ _ (proof.p1 _ _)       := true
+| _ _ (proof.p2 _ _ _)     := true
+| _ _ (proof.p3 _ _)       := true
+| _ _ (proof.q1 _ _)       := true
+| _ _ (proof.q2 _ _)       := true
+| _ _ (proof.q3 _)         := true
+| _ _ (proof.e1 _)         := true
+| _ _ (proof.e2 _ _)       := true
+| _ _ (proof.e3 _ _ _)     := true
+| _ _ (proof.e4 _ _ _)     := true
+| _ _ (proof.e5 _ _ _)     := true
+| _ _ (proof.GE b)         := b.wellformed
+| _ _ (proof.MP b₁ b₂)     := b₁.wellformed && b₂.wellformed
+| n _ (proof.AX q)         := @primrec_theory.isaxiom _ _ (T^n) (prm n) q
+
+variables [primcodable (formula L)] (T : theory L) [∀ i : ℕ, primrec_theory (T^i)] 
+
+lemma proof_soundness (n : ℕ) (p : formula L) (b : proof n p) : b.wellformed T → T^n ⊢ p :=
+begin
+  induction b; try { simp [proof.wellformed] },
+  case proof.GE : n p b IH { intros h, refine provable.GE (IH h) },
+  case proof.MP : n p q b₁ b₂ IH₁ IH₂ { intros h₁ h₂, refine provable.MP (IH₁ h₁) (IH₂ h₂) },
+  case proof.AX : n p { intros h, refine provable.AX h }
+end
+
+def proof.encode : ∀ {n} {p : formula L}, proof n p → ℕ
+| n p (proof.GE b)         := bit0 $ bit0 b.encode
+| n p (proof.MP b₁ b₂) := bit0 $ bit1 (b₁.encode.mkpair b₂.encode)
+| n p (proof.AX q)           := bit1 $ bit1 (encode q)
+
+inductive provable' (T : theory L) : ℕ → formula L → Prop
+| GE : ∀ {n p}, provable' (n + 1) p → provable' n (∀̇ p)
+| MP : ∀ {n p q}, provable' n (p →̇ q) → provable' n p → provable' n q
+| AX : ∀ {n p}, p ∈ T → provable' n (p^n)
+| p1 : ∀ {n p q}, provable' n (p →̇ q →̇ p)
+| p2 : ∀ {n p q r}, provable' n ((p →̇ q →̇ r) →̇ (p →̇ q) →̇ p →̇ r)
+| p3 : ∀ {n p q}, provable' n ((¬̇p →̇ ¬̇q) →̇ q →̇ p)
+| q1 : ∀ {n p t}, provable' n (∀̇ p →̇ p.rew ι[0 ⇝ t])
+| q2 : ∀ {n p q}, provable' n (∀̇ (p →̇ q) →̇ ∀̇ p →̇∀̇ q)
+| q3 : ∀ {n p}, provable' n (p →̇ ∀̇ (p^1))
+| e1 : ∀ {n t}, provable' n (t =̇ t)
+| e2 : ∀ {n t₁ t₂}, provable' n (t₁ =̇ t₂ →̇ t₂ =̇ t₁)
+| e3 : ∀ {n t₁ t₂ t₃}, provable' n (t₁ =̇ t₂ →̇ t₂ =̇ t₃ →̇ t₁ =̇ t₃)
+| e4 : ∀ {n m} {v₁ v₂ : vecterm L m} {f : L.fn (m+1)},
+    provable' n (v₁ ≡̇ v₂ →̇ vecterm.app f v₁ =̇ vecterm.app f v₂)
+| e5 : ∀ {n m} {v₁ v₂ : vecterm L m} {r : L.pr (m+1)},
+    provable' n (v₁ ≡̇ v₂ →̇ formula.app r v₁ →̇ formula.app r v₂)
+
+lemma proof_completeness (p : formula L) (n : ℕ) : provable' T n p → ∃ (b : proof n p), b.wellformed T = tt :=
+begin
+  intros h,
+  induction h generalizing,
+  case provable'.GE : n p h_p IH { rcases IH with ⟨b, eqn⟩, refine ⟨proof.GE b, by simp[eqn]⟩ },
+  case provable'.MP : n p q h₁ h₂ IH₁ IH₂
+  { rcases IH₁ with ⟨b₁, eqn₁⟩,
+    rcases IH₂ with ⟨b₂, eqn₂⟩,
+    refine ⟨proof.MP b₁ b₂, by simp[eqn₁, eqn₂]⟩ },
+  case provable'.AX : n p h { refine ⟨proof.AX (p^n), _⟩, simp, sorry },
+
+end
+end fopl
